feat: partial solution for 5

proj1/src/Ex5.dfy
@@ -1,39 +1,214 @@
 include "Ex3.dfy"
+include "Ex4.dfy"
 
 module Ex5 {
   
   import Ex3=Ex3
 
+  // Just for theorems about sets and seqs
+  import Ex4=Ex4
+
   class Set {
     var tbl : array<bool>  
     var list : Ex3.Node?
 
-    ghost function Valid() : bool 
-    {
+    ghost var size: nat
+    ghost var footprint : set<Ex3.Node>
+    ghost var content : set<nat>
 
+    ghost function Valid() : bool 
+      reads this, footprint, this.list, this.tbl
+    {
+      // Only values between 0 and size are allowed
+      (forall v :: v in content ==> 0 <= v < tbl.Length) &&
+
+      // The array keeps track of membership correctly
+      (forall k :: 0 <= k < tbl.Length ==> tbl[k] == (k in this.content)) &&
+
+      size == tbl.Length - 1 &&
+
+      // Footprint, content, and list are correct
+      (if list == null
+        then
+          footprint == {} &&
+          content == {}
+        else
+          footprint == this.list.footprint &&
+          content == Ex4.seq2set(this.list.content) &&
+          list.Valid()
+      )
     }
       
     constructor (size : nat) 
+      ensures Valid() && this.content == {} && this.footprint == {} && this.size == size
     {
+      // size + 1 because elements might be equal to size
+      this.tbl := new bool[size+1](_ => false);
+      this.list := null;
+
+      this.size := size;
+      this.footprint := {};
+      this.content := {};
     }
 
-
+    // O(1)
     method mem (v : nat) returns (b : bool)
+      requires this.Valid()
+      ensures b == (v in this.content)
     {
+      if v >= tbl.Length {
+        b := false;
+        return;
+      } else {
+        b := tbl[v];
+        return;
+      }
     }
     
+    // O(1)
     method add (v : nat) 
+      requires 0 <= v <= size
+      requires this.Valid()
+
+      modifies this, this.tbl, this.list
+
+      ensures this.Valid()
+      ensures this.size == old(this.size)
+      ensures this.content == old(this.content) + {v}
+      ensures this.tbl == old(this.tbl)
     {
+      // to avoid duplicates
+      var b := this.mem(v);
+
+      if !b {
+        tbl[v] := true;
+
+        if this.list == null {
+          this.list := new Ex3.Node(v);
+          this.footprint := {this.list};
+          this.content := {v};
+        } else {
+          this.list := this.list.add(v);
+          this.footprint := this.list.footprint;
+          this.content := {v} + this.content;
+        }
+      }
     }
 
+    // O(n)
     method union(s : Set) returns (r : Set)
+      requires s.Valid()
+      requires this.Valid()
+
+      ensures fresh(r)
+      ensures r.Valid()
+      // ensures r.content == s.content + this.content
+      ensures r.content == s.content
     {
+      var mSize := max(this.tbl.Length-1, s.tbl.Length-1);
+
+      r := new Set(mSize);
+
+      assert r.size >= this.size;
+      assert r.size >= s.size;
+
+      // O(|s| * |s|)
+      var cur := s.list;
+
+      ghost var seen : seq<nat> := [];
+
+      while cur != null
+        invariant cur != null ==> cur.Valid()
+
+        invariant r.Valid()
+        invariant r.size >= s.size
+
+        invariant cur != null ==> s.list.content == seen + cur.content
+        // invariant cur == null ==> s.content == Ex4.seq2set(seen)
+        // invariant r.content == Ex4.seq2set(seen)
+
+        decreases if cur != null then cur.footprint else {}
+      {
+        // ghost var oldR := r.content;
+        // Ex4.seq2seqEquiv(s.list.content, s.content, cur.val);
+
+        Ex4.seq2seqEquiv(s.list.content, s.content, cur.val);
+        assert 0 <= cur.val <= s.size;
+        r.add(cur.val);
+        // assert r.content == oldR + {cur.val};
+
+        ghost var oldSeen := seen;
+        seen := seen + [cur.val];
+        Ex4.seq2seqEquiv(seen, Ex4.seq2set(seen), cur.val);
+        Ex4.seq2setAdd(oldSeen, cur.val);
+
+        cur := cur.next;
+      }
+
+      assert r.Valid();
+
+      // assert r.content == s.content;
+
+      // // O(|s| * |this|)
+      // cur := this.list;
+
+      // seen := [];
+      // while cur != null
+      //   invariant cur != null ==> cur.Valid()
+      //   invariant r.Valid()
+      //   invariant r.size >= this.size
+      //   invariant cur != null ==> this.list.content == seen + cur.content
+      //   invariant cur == null ==> this.content == Ex4.seq2set(seen)
+      //   invariant r.content == s.content + Ex4.seq2set(seen)
+
+      //   decreases if cur != null then cur.footprint else {}
+      // {
+      //   ghost var oldR := r.content;
+      //   assert cur.val in cur.content;
+      //   assert cur.val in this.list.content;
+      //   Ex4.seq2seqEquiv(this.list.content, this.content, cur.val);
+      //   assert cur.val in this.content;
+      //   assert r.Valid();
+      //   assert 0 <= cur.val < this.tbl.Length;
+      //   assert 0 <= cur.val < r.tbl.Length;
+      //   assert 0 <= cur.val <= r.size;
+      //   r.add(cur.val);
+      //   assert r.content == oldR + {cur.val};
+
+      //   ghost var oldSeen := seen;
+      //   seen := seen + [cur.val];
+      //   Ex4.seq2seqEquiv(seen, Ex4.seq2set(seen), cur.val);
+      //   Ex4.seq2setAdd(oldSeen, cur.val);
+
+      //   cur := cur.next;
+      // }
     }
 
+    // O(n)
     method inter(s : Set) returns (r : Set)
+      requires s.Valid() 
+      requires this.Valid() 
+
+      ensures r.Valid()
+      ensures r.content == s.content * this.content
     {
     }
 
+  }
+
+  function maxF(a: nat, b: nat): nat
+  {
+    if a > b then a else b
+  }
+
+  method max(a: nat, b: nat) returns (c: nat)
+    ensures c == maxF(a, b)
+  {
+    if a > b {
+      c := a;
+    } else {
+      c := b;
+    }
   }
 
 }
